Source/DafnyCore/DafnyPreludeSetAxiom.bpl
@@ -1,121 +1,95 @@
-function TSet(Ty) : Ty;
-axiom (forall t: Ty :: { TSet(t) } Inv0_TSet(TSet(t)) == t);
-axiom (forall t: Ty :: { TSet(t) }      Tag(TSet(t))      == TagSet);
-
-function Inv0_TSet(Ty) : Ty;
-
-const unique TagSet      : TyTag;
-
-axiom (forall bx : Box ::
-    { $IsBox(bx, TBitvector(0)) }
-    ( $IsBox(bx, TBitvector(0)) ==> $Box($Unbox(bx) : Bv0) == bx && $Is($Unbox(bx) : Set Box, TBitvector(0))));
-
-axiom (forall bx : Box, t : Ty ::
-    { $IsBox(bx, TSet(t)) }
-    ( $IsBox(bx, TSet(t)) ==> $Box($Unbox(bx) : Set Box) == bx && $Is($Unbox(bx) : Set Box, TSet(t))));
-
-axiom (forall v: Set Box, t0: Ty :: { $Is(v, TSet(t0)) }
-  $Is(v, TSet(t0)) <==>
-  (forall bx: Box :: { v[bx] }
-    v[bx] ==> $IsBox(bx, t0)));
-
-axiom (forall v: Set Box, t0: Ty, h: Heap :: { $IsAlloc(v, TSet(t0), h) }
-  $IsAlloc(v, TSet(t0), h) <==>
-  (forall bx: Box :: { v[bx] }
-    v[bx] ==> $IsAllocBox(bx, t0, h)));
-
 // ---------------------------------------------------------------
 // -- Axiomatization of sets -------------------------------------
 // ---------------------------------------------------------------
 
-type Set T = [T]bool;
+type Set = [Box]bool;
 
-function Set#Card<T>(Set T): int;
-axiom (forall<T> s: Set T :: { Set#Card(s) } 0 <= Set#Card(s));
+function Set#Card(Set): int;
+axiom (forall s: Set :: { Set#Card(s) } 0 <= Set#Card(s));
 
-function Set#Empty<T>(): Set T;
-axiom (forall<T> o: T :: { Set#Empty()[o] } !Set#Empty()[o]);
-axiom (forall<T> s: Set T :: { Set#Card(s) }
+function Set#Empty(): Set;
+axiom (forall o: Box :: { Set#Empty()[o] } !Set#Empty()[o]);
+axiom (forall s: Set :: { Set#Card(s) }
   (Set#Card(s) == 0 <==> s == Set#Empty()) &&
-  (Set#Card(s) != 0 ==> (exists x: T :: s[x])));
+  (Set#Card(s) != 0 ==> (exists x: Box :: s[x])));
 
 // the empty set could be of anything
-//axiom (forall<T> t: Ty :: { $Is(Set#Empty() : [T]bool, TSet(t)) } $Is(Set#Empty() : [T]bool, TSet(t)));
+//axiom (forall t: Ty :: { $Is(Set#Empty() : [Box]bool, TSet(t)) } $Is(Set#Empty() : [Box]bool, TSet(t)));
 
-function Set#Singleton<T>(T): Set T;
-axiom (forall<T> r: T :: { Set#Singleton(r) } Set#Singleton(r)[r]);
-axiom (forall<T> r: T, o: T :: { Set#Singleton(r)[o] } Set#Singleton(r)[o] <==> r == o);
-axiom (forall<T> r: T :: { Set#Card(Set#Singleton(r)) } Set#Card(Set#Singleton(r)) == 1);
+function Set#Singleton(Box): Set;
+axiom (forall r: Box :: { Set#Singleton(r) } Set#Singleton(r)[r]);
+axiom (forall r: Box, o: Box :: { Set#Singleton(r)[o] } Set#Singleton(r)[o] <==> r == o);
+axiom (forall r: Box :: { Set#Card(Set#Singleton(r)) } Set#Card(Set#Singleton(r)) == 1);
 
-function Set#UnionOne<T>(Set T, T): Set T;
-axiom (forall<T> a: Set T, x: T, o: T :: { Set#UnionOne(a,x)[o] }
+function Set#UnionOne(Set, Box): Set;
+axiom (forall a: Set, x: Box, o: Box :: { Set#UnionOne(a,x)[o] }
   Set#UnionOne(a,x)[o] <==> o == x || a[o]);
-axiom (forall<T> a: Set T, x: T :: { Set#UnionOne(a, x) }
+axiom (forall a: Set, x: Box :: { Set#UnionOne(a, x) }
   Set#UnionOne(a, x)[x]);
-axiom (forall<T> a: Set T, x: T, y: T :: { Set#UnionOne(a, x), a[y] }
+axiom (forall a: Set, x: Box, y: Box :: { Set#UnionOne(a, x), a[y] }
   a[y] ==> Set#UnionOne(a, x)[y]);
-axiom (forall<T> a: Set T, x: T :: { Set#Card(Set#UnionOne(a, x)) }
+axiom (forall a: Set, x: Box :: { Set#Card(Set#UnionOne(a, x)) }
   a[x] ==> Set#Card(Set#UnionOne(a, x)) == Set#Card(a));
-axiom (forall<T> a: Set T, x: T :: { Set#Card(Set#UnionOne(a, x)) }
+axiom (forall a: Set, x: Box :: { Set#Card(Set#UnionOne(a, x)) }
   !a[x] ==> Set#Card(Set#UnionOne(a, x)) == Set#Card(a) + 1);
 
-function Set#Union<T>(Set T, Set T): Set T;
-axiom (forall<T> a: Set T, b: Set T, o: T :: { Set#Union(a,b)[o] }
+function Set#Union(Set, Set): Set;
+axiom (forall a: Set, b: Set, o: Box :: { Set#Union(a,b)[o] }
   Set#Union(a,b)[o] <==> a[o] || b[o]);
-axiom (forall<T> a, b: Set T, y: T :: { Set#Union(a, b), a[y] }
+axiom (forall a, b: Set, y: Box :: { Set#Union(a, b), a[y] }
   a[y] ==> Set#Union(a, b)[y]);
-axiom (forall<T> a, b: Set T, y: T :: { Set#Union(a, b), b[y] }
+axiom (forall a, b: Set, y: Box :: { Set#Union(a, b), b[y] }
   b[y] ==> Set#Union(a, b)[y]);
-axiom (forall<T> a, b: Set T :: { Set#Union(a, b) }
+axiom (forall a, b: Set :: { Set#Union(a, b) }
   Set#Disjoint(a, b) ==>
     Set#Difference(Set#Union(a, b), a) == b &&
     Set#Difference(Set#Union(a, b), b) == a);
 // Follows from the general union axiom, but might be still worth including, because disjoint union is a common case:
-// axiom (forall<T> a, b: Set T :: { Set#Card(Set#Union(a, b)) }
+// axiom (forall a, b: Set :: { Set#Card(Set#Union(a, b)) }
 //   Set#Disjoint(a, b) ==>
 //     Set#Card(Set#Union(a, b)) == Set#Card(a) + Set#Card(b));
 
-function Set#Intersection<T>(Set T, Set T): Set T;
-axiom (forall<T> a: Set T, b: Set T, o: T :: { Set#Intersection(a,b)[o] }
+function Set#Intersection(Set, Set): Set;
+axiom (forall a: Set, b: Set, o: Box :: { Set#Intersection(a,b)[o] }
   Set#Intersection(a,b)[o] <==> a[o] && b[o]);
 
-axiom (forall<T> a, b: Set T :: { Set#Union(Set#Union(a, b), b) }
+axiom (forall a, b: Set :: { Set#Union(Set#Union(a, b), b) }
   Set#Union(Set#Union(a, b), b) == Set#Union(a, b));
-axiom (forall<T> a, b: Set T :: { Set#Union(a, Set#Union(a, b)) }
+axiom (forall a, b: Set :: { Set#Union(a, Set#Union(a, b)) }
   Set#Union(a, Set#Union(a, b)) == Set#Union(a, b));
-axiom (forall<T> a, b: Set T :: { Set#Intersection(Set#Intersection(a, b), b) }
+axiom (forall a, b: Set :: { Set#Intersection(Set#Intersection(a, b), b) }
   Set#Intersection(Set#Intersection(a, b), b) == Set#Intersection(a, b));
-axiom (forall<T> a, b: Set T :: { Set#Intersection(a, Set#Intersection(a, b)) }
+axiom (forall a, b: Set :: { Set#Intersection(a, Set#Intersection(a, b)) }
   Set#Intersection(a, Set#Intersection(a, b)) == Set#Intersection(a, b));
-axiom (forall<T> a, b: Set T :: { Set#Card(Set#Union(a, b)) }{ Set#Card(Set#Intersection(a, b)) }
+axiom (forall a, b: Set :: { Set#Card(Set#Union(a, b)) }{ Set#Card(Set#Intersection(a, b)) }
   Set#Card(Set#Union(a, b)) + Set#Card(Set#Intersection(a, b)) == Set#Card(a) + Set#Card(b));
 
-function Set#Difference<T>(Set T, Set T): Set T;
-axiom (forall<T> a: Set T, b: Set T, o: T :: { Set#Difference(a,b)[o] }
+function Set#Difference(Set, Set): Set;
+axiom (forall a: Set, b: Set, o: Box :: { Set#Difference(a,b)[o] }
   Set#Difference(a,b)[o] <==> a[o] && !b[o]);
-axiom (forall<T> a, b: Set T, y: T :: { Set#Difference(a, b), b[y] }
+axiom (forall a, b: Set, y: Box :: { Set#Difference(a, b), b[y] }
   b[y] ==> !Set#Difference(a, b)[y] );
-axiom (forall<T> a, b: Set T ::
+axiom (forall a, b: Set ::
   { Set#Card(Set#Difference(a, b)) }
   Set#Card(Set#Difference(a, b)) + Set#Card(Set#Difference(b, a))
   + Set#Card(Set#Intersection(a, b))
     == Set#Card(Set#Union(a, b)) &&
   Set#Card(Set#Difference(a, b)) == Set#Card(a) - Set#Card(Set#Intersection(a, b)));
 
-function Set#Subset<T>(Set T, Set T): bool;
-axiom (forall<T> a: Set T, b: Set T :: { Set#Subset(a,b) }
-  Set#Subset(a,b) <==> (forall o: T :: {a[o]} {b[o]} a[o] ==> b[o]));
-// axiom(forall<T> a: Set T, b: Set T ::
+function Set#Subset(Set, Set): bool;
+axiom (forall a: Set, b: Set :: { Set#Subset(a,b) }
+  Set#Subset(a,b) <==> (forall o: Box :: {a[o]} {b[o]} a[o] ==> b[o]));
+// axiom(forall a: Set, b: Set ::
 //   { Set#Subset(a,b), Set#Card(a), Set#Card(b) }  // very restrictive trigger
 //   Set#Subset(a,b) ==> Set#Card(a) <= Set#Card(b));
 
 
-function Set#Equal<T>(Set T, Set T): bool;
-axiom (forall<T> a: Set T, b: Set T :: { Set#Equal(a,b) }
-  Set#Equal(a,b) <==> (forall o: T :: {a[o]} {b[o]} a[o] <==> b[o]));
-axiom (forall<T> a: Set T, b: Set T :: { Set#Equal(a,b) }  // extensionality axiom for sets
+function Set#Equal(Set, Set): bool;
+axiom (forall a: Set, b: Set :: { Set#Equal(a,b) }
+  Set#Equal(a,b) <==> (forall o: Box :: {a[o]} {b[o]} a[o] <==> b[o]));
+axiom (forall a: Set, b: Set :: { Set#Equal(a,b) }  // extensionality axiom for sets
   Set#Equal(a,b) ==> a == b);
 
-function Set#Disjoint<T>(Set T, Set T): bool;
-axiom (forall<T> a: Set T, b: Set T :: { Set#Disjoint(a,b) }
-  Set#Disjoint(a,b) <==> (forall o: T :: {a[o]} {b[o]} !a[o] || !b[o]));
+function Set#Disjoint(Set, Set): bool;
+axiom (forall a: Set, b: Set :: { Set#Disjoint(a,b) }
+  Set#Disjoint(a,b) <==> (forall o: Box :: {a[o]} {b[o]} !a[o] || !b[o]));
