Source/DafnyCore/DafnyPreludeTyDt.bpl
@@ -15,74 +15,24 @@ const $$Language$Dafny: bool uses {  // To be recognizable to the ModelViewer as
 // -- Types ------------------------------------------------------
 // ---------------------------------------------------------------
 
-type Ty;
 type Bv0 = int;
+type ClassTag;
 
-const unique TBool : Ty uses {
-  axiom Tag(TBool) == TagBool;
+datatype Ty {
+  TBool(),
+  TChar(),
+  TInt(),
+  TReal(),
+  TORDINAL(),
+  TBitvector(len: int),
+  TSet(elemTy: Ty),
+  TISet(elemTy: Ty),
+  TMultiSet(elemTy: Ty),
+  TSeq(elemTy: Ty),
+  TMap(keyTy: Ty, elemTy: Ty),
+  TIMap(keyTy: Ty, elemTy: Ty),
+  TClass(tag: ClassTag)
 }
-const unique TChar : Ty uses {
-  axiom Tag(TChar) == TagChar;
-}
-const unique TInt  : Ty uses {
-  axiom Tag(TInt) == TagInt;
-}
-const unique TReal : Ty uses {
-  axiom Tag(TReal) == TagReal;
-}
-const unique TORDINAL  : Ty uses {
-  axiom Tag(TORDINAL) == TagORDINAL;
-}
-// See for which axioms we can make use of the trigger to determine the connection.
-function TBitvector(int) : Ty;
-axiom (forall w: int :: { TBitvector(w) } Inv0_TBitvector(TBitvector(w)) == w);
-
-function Inv0_TBitvector(Ty) : int;
-
-function TSet(Ty) : Ty;
-axiom (forall t: Ty :: { TSet(t) } Inv0_TSet(TSet(t)) == t);
-axiom (forall t: Ty :: { TSet(t) }      Tag(TSet(t))      == TagSet);
-
-function Inv0_TSet(Ty) : Ty;
-
-const unique TagSet : TyTag;
-
-axiom (forall bx : Box ::
-    { $IsBox(bx, TBitvector(0)) }
-    ( $IsBox(bx, TBitvector(0)) ==> $Box($Unbox(bx) : Bv0) == bx && $Is($Unbox(bx) : Set, TBitvector(0))));
-
-axiom (forall bx : Box, t : Ty ::
-    { $IsBox(bx, TSet(t)) }
-    ( $IsBox(bx, TSet(t)) ==> $Box($Unbox(bx) : Set) == bx && $Is($Unbox(bx) : Set, TSet(t))));
-
-axiom (forall v: Set, t0: Ty :: { $Is(v, TSet(t0)) }
-  $Is(v, TSet(t0)) <==>
-  (forall bx: Box :: { v[bx] }
-    v[bx] ==> $IsBox(bx, t0)));
-
-#if USE_HEAP
-axiom (forall v: Set, t0: Ty, h: Heap :: { $IsAlloc(v, TSet(t0), h) }
-  $IsAlloc(v, TSet(t0), h) <==>
-  (forall bx: Box :: { v[bx] }
-    v[bx] ==> $IsAllocBox(bx, t0, h)));
-#endif
-
-// -- Classes and Datatypes --
-
-// -- Type Tags --
-type TyTag;
-function Tag(Ty) : TyTag;
-
-const unique TagBool     : TyTag;
-const unique TagChar     : TyTag;
-const unique TagInt      : TyTag;
-const unique TagReal     : TyTag;
-const unique TagORDINAL  : TyTag;
-
-const unique TagClass    : TyTag;
-
-type TyTagFamily;
-function TagFamily(Ty): TyTagFamily;
 
 #if !USE_SETS
 type Set = [Box]bool;
@@ -178,17 +128,17 @@ function $IsBox<T>(T,Ty): bool;
 function $IsAllocBox<T>(T,Ty,Heap): bool;
 
 axiom (forall bx : Box ::
-    { $IsBox(bx, TInt) }
-    ( $IsBox(bx, TInt) ==> $Box($Unbox(bx) : int) == bx && $Is($Unbox(bx) : int, TInt)));
+    { $IsBox(bx, TInt()) }
+    ( $IsBox(bx, TInt()) ==> $Box($Unbox(bx) : int) == bx && $Is($Unbox(bx) : int, TInt())));
 axiom (forall bx : Box ::
-    { $IsBox(bx, TReal) }
-    ( $IsBox(bx, TReal) ==> $Box($Unbox(bx) : real) == bx && $Is($Unbox(bx) : real, TReal)));
+    { $IsBox(bx, TReal()) }
+    ( $IsBox(bx, TReal()) ==> $Box($Unbox(bx) : real) == bx && $Is($Unbox(bx) : real, TReal())));
 axiom (forall bx : Box ::
-    { $IsBox(bx, TBool) }
-    ( $IsBox(bx, TBool) ==> $Box($Unbox(bx) : bool) == bx && $Is($Unbox(bx) : bool, TBool)));
+    { $IsBox(bx, TBool()) }
+    ( $IsBox(bx, TBool()) ==> $Box($Unbox(bx) : bool) == bx && $Is($Unbox(bx) : bool, TBool())));
 axiom (forall bx : Box ::
-    { $IsBox(bx, TChar) }
-    ( $IsBox(bx, TChar) ==> $Box($Unbox(bx) : char) == bx && $Is($Unbox(bx) : char, TChar)));
+    { $IsBox(bx, TChar()) }
+    ( $IsBox(bx, TChar()) ==> $Box($Unbox(bx) : char) == bx && $Is($Unbox(bx) : char, TChar())));
 
 // Since each bitvector type is a separate type in Boogie, the Box/Unbox axioms for bitvectors are
 // generated programmatically. Except, Bv0 is given here.
@@ -207,11 +157,11 @@ axiom (forall<T> v : T, t : Ty, h : Heap ::
 // Type-argument to $Is is the /representation type/,
 // the second value argument to $Is is the actual type.
 function $Is<T>(T,Ty): bool;           // no heap for now
-axiom(forall v : int  :: { $Is(v,TInt) }  $Is(v,TInt));
-axiom(forall v : real :: { $Is(v,TReal) } $Is(v,TReal));
-axiom(forall v : bool :: { $Is(v,TBool) } $Is(v,TBool));
-axiom(forall v : char :: { $Is(v,TChar) } $Is(v,TChar));
-axiom(forall v : ORDINAL :: { $Is(v,TORDINAL) } $Is(v,TORDINAL));
+axiom(forall v : int  :: { $Is(v,TInt()) }  $Is(v,TInt()));
+axiom(forall v : real :: { $Is(v,TReal()) } $Is(v,TReal()));
+axiom(forall v : bool :: { $Is(v,TBool()) } $Is(v,TBool()));
+axiom(forall v : char :: { $Is(v,TChar()) } $Is(v,TChar()));
+axiom(forall v : ORDINAL :: { $Is(v,TORDINAL()) } $Is(v,TORDINAL()));
 
 // Since every bitvector type is a separate type in Boogie, the $Is/$IsAlloc axioms
 // for bitvectors are generated programatically. Except, TBitvector(0) is given here.
@@ -219,11 +169,11 @@ axiom (forall v: Bv0 :: { $Is(v, TBitvector(0)) } $Is(v, TBitvector(0)));
 
 #if USE_HEAP
 function $IsAlloc<T>(T,Ty,Heap): bool;
-axiom(forall h : Heap, v : int  :: { $IsAlloc(v,TInt,h) }  $IsAlloc(v,TInt,h));
-axiom(forall h : Heap, v : real :: { $IsAlloc(v,TReal,h) } $IsAlloc(v,TReal,h));
-axiom(forall h : Heap, v : bool :: { $IsAlloc(v,TBool,h) } $IsAlloc(v,TBool,h));
-axiom(forall h : Heap, v : char :: { $IsAlloc(v,TChar,h) } $IsAlloc(v,TChar,h));
-axiom(forall h : Heap, v : ORDINAL :: { $IsAlloc(v,TORDINAL,h) } $IsAlloc(v,TORDINAL,h));
+axiom(forall h : Heap, v : int  :: { $IsAlloc(v,TInt(),h) }  $IsAlloc(v,TInt(),h));
+axiom(forall h : Heap, v : real :: { $IsAlloc(v,TReal(),h) } $IsAlloc(v,TReal(),h));
+axiom(forall h : Heap, v : bool :: { $IsAlloc(v,TBool(),h) } $IsAlloc(v,TBool(),h));
+axiom(forall h : Heap, v : char :: { $IsAlloc(v,TChar(),h) } $IsAlloc(v,TChar(),h));
+axiom(forall h : Heap, v : ORDINAL :: { $IsAlloc(v,TORDINAL(),h) } $IsAlloc(v,TORDINAL(),h));
     
 axiom (forall v: Bv0, h: Heap :: { $IsAlloc(v, TBitvector(0), h) } $IsAlloc(v, TBitvector(0), h));
 
@@ -271,15 +221,11 @@ axiom (forall a: ClassName, b: ClassName :: { TypeTuple(a,b) }
 
 type HandleType;
 
-#if USE_HEAP
 function SetRef_to_SetBox(s: [ref]bool): Set;
 axiom (forall s: [ref]bool, bx: Box :: { SetRef_to_SetBox(s)[bx] }
   SetRef_to_SetBox(s)[bx] == s[$Unbox(bx): ref]);
 axiom (forall s: [ref]bool :: { SetRef_to_SetBox(s) }
   $Is(SetRef_to_SetBox(s), TSet(Tclass._System.object?())));
-#else
-function SetRef_to_SetBox(s: [ref]bool): [Box]bool;
-#endif
 
 // Functions ApplyN, RequiresN, and ReadsN are generated on demand by the translator,
 // but Apply1 is referred to in the prelude, so its definition is hardcoded here.
@@ -558,7 +504,7 @@ procedure $IterHavoc1(this: ref, modi: Set, nw: Set);
               $o == this || modi[$Box($o)] || nw[$Box($o)]);
   ensures $HeapSucc(old($Heap), $Heap);
 
-procedure $IterCollectNewObjects(prevHeap: Heap, newHeap: Heap, this: ref, NW: Field (Set))
+procedure $IterCollectNewObjects(prevHeap: Heap, newHeap: Heap, this: ref, NW: Field Set)
                         returns (s: Set);
   ensures (forall bx: Box :: { s[bx] } s[bx] <==>
               (read(newHeap, this, NW) : Set)[bx] ||
